src/spec/TLS13.ConnectionState.ProtectedWireLemmas.fsti
@@ -2806,6 +2806,209 @@ val lemma_protected_handshake_event_projection_pairs_after_server_write_client_r
             client_tail_received
             client_final)
 
+val lemma_protected_handshake_event_projection_pairs_after_server_write_client_read_install_two_heads_then_both_non_install_local_heads_with_next_alignment_and_tails
+  (server:CS.connection_model)
+  (client:CS.connection_model)
+  (server_after_install:CS.connection_model)
+  (client_after_install:CS.connection_model)
+  (server_after0:CS.connection_model)
+  (client_after0:CS.connection_model)
+  (server_after1:CS.connection_model)
+  (client_after1:CS.connection_model)
+  (server_after_skip:CS.connection_model)
+  (client_after_skip:CS.connection_model)
+  (server_after2:CS.connection_model)
+  (client_after2:CS.connection_model)
+  (server_skip:CS.local_event)
+  (client_skip:CS.local_event)
+  (server_material:CS.traffic_key_material)
+  (client_material:CS.traffic_key_material)
+  (sent_msg0:M.handshake_msg)
+  (received_msg0:M.handshake_msg)
+  (sent_msg1:M.handshake_msg)
+  (received_msg1:M.handshake_msg)
+  (sent_msg2:M.handshake_msg)
+  (received_msg2:M.handshake_msg)
+  (server_rest:list CS.conn_event)
+  (client_rest:list CS.conn_event)
+  (server_raw_sent:B.bytes)
+  (server_raw_received:B.bytes)
+  (client_raw_sent:B.bytes)
+  (client_raw_received:B.bytes)
+  (server_final:CS.connection_model)
+  (client_final:CS.connection_model)
+  : Lemma
+      (requires
+        (match
+          server.CS.model_handshake.CS.hs_keys.CS.ks_handshake_secret,
+          client.CS.model_handshake.CS.hs_keys.CS.ks_handshake_secret
+        with
+        | Some server_secret, Some client_secret ->
+          Seq.equal server_secret client_secret
+        | _, _ ->
+          False) /\
+        Seq.equal
+          server.CS.model_handshake.CS.hs_transcript
+          client.CS.model_handshake.CS.hs_transcript /\
+        local_event_does_not_install_record_keys server_skip /\
+        local_event_does_not_install_record_keys client_skip /\
+        Seq.equal server_raw_sent client_raw_received /\
+        protected_handshake_wire_round_trip_message sent_msg0 /\
+        protected_handshake_wire_round_trip_message received_msg0 /\
+        protected_handshake_wire_round_trip_message sent_msg1 /\
+        protected_handshake_wire_round_trip_message received_msg1 /\
+        protected_handshake_wire_round_trip_message sent_msg2 /\
+        protected_handshake_wire_round_trip_message received_msg2 /\
+        CS.step_model
+          server
+          (CS.ConnLocalEvent
+            (CS.LocalInstallTrafficKeysForRole {
+              CS.install_role = CS.ServerEndpoint;
+              CS.install_payload = {
+                CS.install_epoch = CS.TrafficHandshake;
+                CS.install_direction = CS.TrafficWrite;
+                CS.install_material = server_material;
+              };
+            })) == Some server_after_install /\
+        CS.step_model
+          client
+          (CS.ConnLocalEvent
+            (CS.LocalInstallTrafficKeys {
+              CS.install_epoch = CS.TrafficHandshake;
+              CS.install_direction = CS.TrafficRead;
+              CS.install_material = client_material;
+            })) == Some client_after_install /\
+        CS.step_model
+          server_after_install
+          (CS.ConnNetworkEvent {
+            CL.message_direction = CL.Sent;
+            CL.message_value = M.TlsHandshake sent_msg0;
+          }) == Some server_after0 /\
+        CS.step_model
+          client_after_install
+          (CS.ConnNetworkEvent {
+            CL.message_direction = CL.Received;
+            CL.message_value = M.TlsHandshake received_msg0;
+          }) == Some client_after0 /\
+        server_after0.CS.model_record.CS.record_write ==
+          R.next_seq server_after_install.CS.model_record.CS.record_write /\
+        client_after0.CS.model_record.CS.record_read ==
+          R.next_seq client_after_install.CS.model_record.CS.record_read /\
+        CS.step_model
+          server_after0
+          (CS.ConnNetworkEvent {
+            CL.message_direction = CL.Sent;
+            CL.message_value = M.TlsHandshake sent_msg1;
+          }) == Some server_after1 /\
+        CS.step_model
+          client_after0
+          (CS.ConnNetworkEvent {
+            CL.message_direction = CL.Received;
+            CL.message_value = M.TlsHandshake received_msg1;
+          }) == Some client_after1 /\
+        server_after1.CS.model_record.CS.record_write ==
+          R.next_seq server_after0.CS.model_record.CS.record_write /\
+        client_after1.CS.model_record.CS.record_read ==
+          R.next_seq client_after0.CS.model_record.CS.record_read /\
+        CS.step_model server_after1 (CS.ConnLocalEvent server_skip) ==
+          Some server_after_skip /\
+        CS.step_model client_after1 (CS.ConnLocalEvent client_skip) ==
+          Some client_after_skip /\
+        CS.step_model
+          server_after_skip
+          (CS.ConnNetworkEvent {
+            CL.message_direction = CL.Sent;
+            CL.message_value = M.TlsHandshake sent_msg2;
+          }) == Some server_after2 /\
+        CS.step_model
+          client_after_skip
+          (CS.ConnNetworkEvent {
+            CL.message_direction = CL.Received;
+            CL.message_value = M.TlsHandshake received_msg2;
+          }) == Some client_after2 /\
+        server_after2.CS.model_record.CS.record_write ==
+          R.next_seq server_after_skip.CS.model_record.CS.record_write /\
+        client_after2.CS.model_record.CS.record_read ==
+          R.next_seq client_after_skip.CS.model_record.CS.record_read /\
+        CS.conn_events_sent_seal_replay
+          server
+          (CS.ConnLocalEvent
+            (CS.LocalInstallTrafficKeysForRole {
+              CS.install_role = CS.ServerEndpoint;
+              CS.install_payload = {
+                CS.install_epoch = CS.TrafficHandshake;
+                CS.install_direction = CS.TrafficWrite;
+                CS.install_material = server_material;
+              };
+            }) :: CS.ConnNetworkEvent {
+              CL.message_direction = CL.Sent;
+              CL.message_value = M.TlsHandshake sent_msg0;
+            } :: CS.ConnNetworkEvent {
+              CL.message_direction = CL.Sent;
+              CL.message_value = M.TlsHandshake sent_msg1;
+            } :: CS.ConnLocalEvent server_skip :: CS.ConnNetworkEvent {
+              CL.message_direction = CL.Sent;
+              CL.message_value = M.TlsHandshake sent_msg2;
+            } :: server_rest)
+          server_raw_sent
+          server_raw_received
+          server_final /\
+        CS.conn_events_received_decode_replay
+          client
+          (CS.ConnLocalEvent
+            (CS.LocalInstallTrafficKeys {
+              CS.install_epoch = CS.TrafficHandshake;
+              CS.install_direction = CS.TrafficRead;
+              CS.install_material = client_material;
+            }) :: CS.ConnNetworkEvent {
+              CL.message_direction = CL.Received;
+              CL.message_value = M.TlsHandshake received_msg0;
+            } :: CS.ConnNetworkEvent {
+              CL.message_direction = CL.Received;
+              CL.message_value = M.TlsHandshake received_msg1;
+            } :: CS.ConnLocalEvent client_skip :: CS.ConnNetworkEvent {
+              CL.message_direction = CL.Received;
+              CL.message_value = M.TlsHandshake received_msg2;
+            } :: client_rest)
+          client_raw_sent
+          client_raw_received
+          client_final)
+      (ensures
+        exists pair0 pair1 pair2 server_tail_sent server_tail_received
+          client_tail_sent client_tail_received.
+          pair0.pm_sender == server_after_install /\
+          pair0.pm_receiver == client_after_install /\
+          protected_handshake_event_projection_pair
+            pair0
+            sent_msg0
+            received_msg0 /\
+          pair1.pm_sender == server_after0 /\
+          pair1.pm_receiver == client_after0 /\
+          protected_handshake_event_projection_pair
+            pair1
+            sent_msg1
+            received_msg1 /\
+          pair2.pm_sender == server_after_skip /\
+          pair2.pm_receiver == client_after_skip /\
+          protected_handshake_event_projection_pair
+            pair2
+            sent_msg2
+            received_msg2 /\
+          write_read_record_material_aligned server_after2 client_after2 /\
+          Seq.equal server_tail_sent client_tail_received /\
+          CS.conn_events_sent_seal_replay
+            server_after2
+            server_rest
+            server_tail_sent
+            server_tail_received
+            server_final /\
+          CS.conn_events_received_decode_replay
+            client_after2
+            client_rest
+            client_tail_sent
+            client_tail_received
+            client_final)
+
 val lemma_protected_handshake_event_projection_pair_after_client_write_server_read_install_heads_with_tails
   (client:CS.connection_model)
   (server:CS.connection_model)
